FunMaps.v
@@ -41,8 +41,17 @@ Ltac reduction :=
     destruct (H1 A) as [HA HB]; clear H1;
     let HC := fresh "HC" in
     let HD := fresh "HD" in
-    destruct (HA _ H2) as [cblk [HC HD]]; clear HA HB H2;
-    exists cblk
+    let cblk := fresh "cblk" in
+    destruct (HA _ H2) as [cblk [HC HD]]; clear HA HB H2
+  | [ H1 : SetMap_AbsR _ _ _,
+      H2 : In _ (relEns ?K) (?A, ?D) |- _ ] =>
+    let HA := fresh "HA" in
+    let HB := fresh "HB" in
+    destruct (H1 A) as [HA HB]; clear H1;
+    let HC := fresh "HC" in
+    let HD := fresh "HD" in
+    let cblk := fresh "cblk" in
+    destruct (HA _ H2) as [cblk [HC HD]]; clear HA HB H2
   | [ H1 : SetMap_AbsR _ _ _,
       H2 : M.find ?A ?K = Some ?D |- _ ] =>
     let HA := fresh "HA" in
@@ -50,8 +59,8 @@ Ltac reduction :=
     destruct (H1 A) as [HA HB]; clear H1;
     let HC := fresh "HC" in
     let HD := fresh "HD" in
-    destruct (HB _ H2) as [blk [HC HD]]; clear HA HB H2;
-    exists blk
+    let blk := fresh "blk" in
+    destruct (HB _ H2) as [blk [HC HD]]; clear HA HB H2
   end.
 
 Section FunMaps_AbsR.
@@ -62,41 +71,40 @@ Variable or : FunRel M.key A.
 Variable nr : M.t B.
 Variable H  : SetMap_AbsR or nr R.
 
-Hypothesis Oeq_eq : forall a b, O.eq a b -> a = b.
-
-Lemma Find_find_if P P' a b b' :
-  (forall i a b, R a b -> P i a <-> is_true (P' i b))
+Lemma SetMap_AbsR_prj1 : forall (addr : M.key) (blk : A) cblk,
+  Ensembles.In _ (relEns or) (addr, blk)
     -> (forall a b c, R a b -> R a c -> b = c)
-    -> (forall (a b : M.key) (x y : B),
-          is_true (P' a x) -> ~ M.E.eq a b -> P' b y = false)
-    -> R b b'
-    -> Find P a b or
-    -> find_if P' nr = Some (a, b').
+    -> R blk cblk
+    -> M.find (elt:=B) addr nr = Some cblk.
 Proof.
   intros.
-  destruct H4.
-  eapply H0 in H5; eauto; clear H0.
-  destruct (H a) as [H0 _]; clear H.
-  destruct (H0 _ H4) as [b'' [H H6]]; clear H4 H0.
-  unfold find_if.
-  rewrite F.elements_o in H.
-  rewrite M.fold_1.
-  induction (M.elements nr).
-    discriminate.
-  rewrite fold_Some_cons; auto.
-  destruct a0; simpl in *.
-  unfold F.eqb in H.
-  destruct (F.eq_dec a k).
-    pose proof (H1 _ _ _ H3 H6); subst.
-    clear H1 H2 H3 H6 IHl.
-    inversion H; clear H.
-    unfold M.E.eq in e.
-    apply Oeq_eq in e; subst.
-    rewrite H5.
-    reflexivity.
-  rewrite (IHl H), (H2 _ _ _ _ H5 n).
-  reflexivity.
+  destruct (H addr); clear H.
+  destruct (H3 _ H0) as [cblk' [? ?]]; clear H0 H3.
+  rewrite (H1 _ _ _ H2 H5); assumption.
 Qed.
+
+Lemma SetMap_AbsR_prj1_ex : forall (addr : M.key) (blk : A),
+  Ensembles.In _ (relEns or) (addr, blk)
+    -> exists cblk : B,
+         M.find (elt:=B) addr nr = Some cblk /\ R blk cblk.
+Proof.
+  intros.
+  destruct (H addr); clear H.
+  destruct (H1 _ H0) as [cblk [? ?]]; clear H0 H1.
+  exists cblk; auto.
+Qed.
+
+Lemma SetMap_AbsR_prj2_ex : forall (addr : M.key) (cblk : B),
+  M.find (elt:=B) addr nr = Some cblk
+    -> exists blk : A, Lookup addr blk or /\ R blk cblk.
+Proof.
+  intros.
+  destruct (H addr); clear H.
+  destruct (H2 _ H0) as [blk [? ?]]; clear H0 H2.
+  exists blk; auto.
+Qed.
+
+Hypothesis Oeq_eq : forall a b, O.eq a b -> a = b.
 
 Lemma Update_SetMap_AbsR : forall k v v',
   R v v' -> SetMap_AbsR (Update k v or) (M.add k v' nr) R.
@@ -107,6 +115,7 @@ Proof.
       split; trivial.
       apply F.find_mapsto_iff, F.add_mapsto_iff.
       left; auto.
+    exists cblk.
     intuition.
     apply F.find_mapsto_iff in HC.
     apply F.find_mapsto_iff, F.add_mapsto_iff.
@@ -118,7 +127,8 @@ Proof.
     apply Oeq_eq in H1; subst.
     right; constructor.
   apply F.find_mapsto_iff in H2.
-  reduction; intuition.
+  reduction; exists blk.
+  intuition.
   left; constructor; auto.
   unfold Ensembles.In; simpl.
   unfold not; intros.
@@ -129,7 +139,7 @@ Lemma Remove_SetMap_AbsR : forall k,
   SetMap_AbsR (Remove k or) (M.remove k nr) R.
 Proof.
   split; intros.
-    reduction.
+    reduction; exists cblk.
     intuition.
     apply F.find_mapsto_iff, F.remove_mapsto_iff.
     split; auto.
@@ -138,7 +148,7 @@ Proof.
   apply F.find_mapsto_iff, F.remove_mapsto_iff in H0.
   destruct H0.
   apply F.find_mapsto_iff in H1.
-  reduction.
+  reduction; exists blk.
   intuition.
   constructor; trivial.
   unfold Ensembles.In; simpl.
@@ -179,6 +189,97 @@ Proof.
   intros.
   apply Oeq_eq in H2.
   subst; reflexivity.
+Qed.
+
+Lemma Proper_Oeq_negb : forall f,
+  Proper (O.eq ==> eq ==> eq) f ->
+  Proper (O.eq ==> eq ==> eq) (fun (k : M.key) (e : B) => negb (f k e)).
+Proof.
+  intros.
+  intros x y H1 x' y' H2. subst.
+  apply Oeq_eq in H1; subst.
+  reflexivity.
+Qed.
+
+Lemma Partition_SetMap_AbsR
+      (f : M.key -> A -> Prop)
+      (f' : M.key -> B -> bool)
+      (f'_Proper : Proper (O.eq ==> eq ==> eq) f')  :
+  (forall a b, R a b -> forall i, Bool.reflect (f i a) (f' i b))
+    -> forall a a', Partition f or = (a, a')
+    -> forall b b', P.partition f' nr = (b, b')
+    -> SetMap_AbsR a b R /\ SetMap_AbsR a' b' R.
+Proof.
+  split; intros; split; intros.
+  - unfold Partition in H0.
+    unfold P.partition in H1.
+    inversion H0; subst; clear H0;
+    inversion H1; subst; clear H1;
+    simpl in H2; destruct H2.
+    destruct (H addr) as [H3 _].
+    destruct (H3 _ H1) as [cblk [? ?]]; clear H1 H3.
+    exists cblk; intuition.
+    apply F.find_mapsto_iff.
+    apply F.find_mapsto_iff in H2.
+    apply P.filter_iff; intuition.
+    destruct (X _ _ H4 addr); intuition.
+Admitted.
+(*
+  - destruct (H addr); clear H H1.
+    apply F.find_mapsto_iff in H0.
+    apply P.filter_iff in H0; trivial.
+    destruct H0.
+    apply F.find_mapsto_iff in H.
+    destruct (H2 _ H) as [blk [? ?]]; clear H H2.
+    exists blk; intuition.
+    split; intuition.
+    destruct (X _ _ H3 addr); intuition.
+  - destruct (H addr); clear H H2.
+    destruct H0.
+    destruct (H1 _ H0) as [cblk [? ?]]; clear H0 H1.
+    exists cblk; intuition.
+    apply F.find_mapsto_iff.
+    apply F.find_mapsto_iff in H2.
+    apply P.filter_iff; intuition.
+    apply Proper_Oeq_negb; assumption.
+    apply negb_true_iff.
+    destruct (X _ _ H3 addr); intuition.
+  - destruct (H addr); clear H H1.
+    apply F.find_mapsto_iff in H0.
+    apply P.filter_iff in H0; trivial.
+    destruct H0.
+    apply negb_true_iff in H0.
+    apply F.find_mapsto_iff in H.
+    destruct (H2 _ H) as [blk [? ?]]; clear H H2.
+    exists blk; intuition.
+    split; intuition.
+      destruct (X _ _ H3 addr); intuition.
+    apply Proper_Oeq_negb; assumption.
+Qed.
+*)
+
+Lemma Same_set_SetMap_AbsR : forall a b r HF,
+  Same_set _ (relEns a) b
+    -> SetMap_AbsR a r R
+    -> SetMap_AbsR (mkFunRel b HF) r R.
+Proof.
+  intros.
+  intros addr.
+  destruct (H1 addr); clear H1.
+  split; intros.
+    unfold Lookup in H1.
+    unfold Same_set, Included in H0.
+    destruct H0.
+    apply H4 in H1.
+    destruct (H2 _ H1) as [cblk [? ?]].
+    exists cblk.
+    intuition.
+  destruct (H3 _ H1) as [blk [? ?]].
+  exists blk.
+  unfold Same_set, Included in H0.
+  destruct H0.
+  apply H0 in H4.
+  intuition.
 Qed.
 
 End FunMaps_AbsR.
